pulse/share/steel/examples/pulse/lib/Pulse.Lib.HashTable.fsti
@@ -41,31 +41,55 @@ val models #k #v (ht:ht_t k v) (pht:pht_t k v) : vprop
 
 let pht_sz #k #v (pht:pht_t k v) : GTot pos = pht.repr.sz
 
+val alloc (#k:eqtype) (#v:Type0) (hashf:k -> US.t) (l:pos_us)
+  : stt (ht_t k v) emp 
+        (fun ht ->
+          exists_ (fun pht ->
+            models ht pht **
+            pure (pht == mk_init_pht hashf l)))
+
+val dealloc (#k:eqtype) (#v:Type0) (ht:ht_t k v)
+  : stt unit (requires exists_ (fun pht -> models ht pht))
+             (ensures fun _ -> emp)
+
+val lookup (#kt:eqtype) (#vt:Type0)
+           (ht:ht_t kt vt) (k:kt)
+           (#pht:erased (pht_t kt vt))
+  : stt (bool & option vt)
+    (models ht pht)
+    (fun p -> models ht pht ** pure (fst p ==> (snd p) == PHT.lookup pht k ))
+
+val insert (#kt:eqtype) (#vt:Type0)
+           (ht:ht_t kt vt) (k:kt) (v:vt)
+           (#pht:erased (pht_t kt vt){PHT.not_full pht.repr})
+  : stt bool 
+        (models ht pht)
+        (fun b -> 
+          exists_ (fun pht' -> 
+            models ht pht' **
+            pure (if b
+                  then pht'==PHT.insert pht k v
+                  else pht'==reveal pht)))
+
+
+val delete (#kt:eqtype) (#vt:Type0)
+           (ht:ht_t kt vt) (k:kt)
+           (#pht:erased (pht_t kt vt))
+  : stt bool
+    (models ht pht)
+    (fun b -> 
+        exists_ (fun pht' -> 
+            models ht pht' **
+            pure (if b
+                  then pht'==PHT.delete pht k
+                  else pht'==reveal pht)))
+
+val not_full (#kt:eqtype) (#vt:eqtype)
+             (ht:ht_t kt vt)
+             (#pht:erased (pht_t kt vt))
+  : stt bool (models ht pht)
+      (fun b -> 
+        models ht pht ** 
+        pure (b ==> PHT.not_full pht.repr))
 
 val test_mono (_:unit) : stt unit emp (fun _ -> emp)
-// let maybe_update #kt #vt (b:bool) (ht:ht_t kt vt) (pht pht':pht_t kt vt)
-//   : vprop
-//   = if b then models ht pht' else models ht pht
-
-// val insert (#kt:eqtype) (#vt:Type0)
-//            (#pht:(p:erased (pht_t kt vt){PHT.not_full p.repr}))
-//            (ht:ht_t kt vt) (k:kt) (v:vt)
-//   : stt bool 
-//     (models ht pht)
-//     (fun b -> maybe_update b ht pht (PHT.insert pht k v))
-
-// val delete (#kt:eqtype) (#vt:Type0)
-//            (#pht:erased (pht_t kt vt))
-//            (ht:ht_t kt vt) (k:kt)
-//   : stt bool
-//     (models ht pht)
-//     (fun b -> maybe_update b ht pht (PHT.delete pht k))
-
-// val not_full (#kt:eqtype) (#vt:Type0)
-//              (#pht:erased (pht_t kt vt))
-//              (ht:ht_t kt vt)
-//   : stt bool
-//     (models ht pht)
-//     (fun b -> 
-//       models ht pht ** 
-//       pure (b ==> PHT.not_full pht.repr))
